What is the group action on initial moves for the tensor product?

AsynchronousGames.v
@@ -15,6 +15,12 @@ Record PartialOrder :=
     reflexive : forall (x : M), leq x x;
     anti_symmetric : forall (x y : M), leq x y /\ leq y x -> x = y;
     transitive : forall (x y z : M), leq x y /\ leq y z -> leq x z;
+
+    unit_is_least : forall i i' m, 
+    leq (existT _ i (inl tt)) (existT _ i' m) <-> i = i';
+
+    leq_same_component : forall i i' m m',
+    leq (existT _ i m) (existT _ i' m') -> i = i';
   }.
 
 Record EventStructure := 
@@ -32,28 +38,9 @@ Record EventStructure :=
 
 Definition Position (E : EventStructure) := list (M (P E)).
 
-Definition valid_position (E : EventStructure) (p : Position E) :=
-forall m n, (In n p -> leq (P E) m n -> In m p)
-/\
-(In m p /\ In n p ->  not (incompatible E m n)).
-
-Definition move_from (E : EventStructure) (m : (M (P E))) (p q: Position E) :=
-(In m q) /\ (~ In m p) /\ (forall n, In n p -> In n q).
-
 Definition Path (E: EventStructure) := prod (Position E) (list (M (P E))).
 
-Definition valid_path (E: EventStructure) (p : Path E) :=
-forall n, 0 <= n <= length (snd p) ->
-(valid_position E ((fst p) ++ (firstn n (snd p))) /\
-(n > 0 -> (exists m, (nth_error (snd p) (n-1)) = Some m /\
-move_from E m ((fst p) ++ (firstn (n-1) (snd p)))
-((fst p) ++ (firstn n (snd p)))))).
-
 Definition Walk (E: EventStructure) := prod (Path E) (Path E).
-
-Definition valid_walk (E: EventStructure) (w : Walk E) := 
-valid_path E (fst w) /\ valid_path E (snd w) /\
-(forall x,  In x (fst (fst w)) <-> In x (fst (snd w))).
 
 Inductive Infinity : Type :=
 | plus_infinity : Infinity
@@ -66,8 +53,23 @@ Inductive InfinitePosition (E : EventStructure) : Type :=
 Definition initial_move (P : PartialOrder) (m : M P) :=
 forall n, leq P n m -> n = m.
 
+Fact initial_is_unit :
+forall E m, initial_move E m <->
+(exists i, m = existT _ i (inl tt)).
+Proof. unfold iff. split.
++ intros. unfold initial_move in H. destruct m. 
+refine (ex_intro _ x _). symmetry. apply H.
+apply unit_is_least. auto.
++ intros. unfold initial_move. intros. destruct H. subst.
+apply anti_symmetric. split.
+++ auto.
+++ destruct n. apply leq_same_component in H0. subst. 
+apply unit_is_least. auto.
+Qed.
+
 Definition second_move (P : PartialOrder) (m : M P) :=
-(~ initial_move P m) /\ (forall n, leq P n m -> initial_move P n).
+(~ initial_move P m) /\ 
+(forall n, (leq P n m /\ (n <> m)) -> initial_move P n).
 
 Record AsynchronousArena := {
     E : EventStructure;
@@ -85,17 +87,16 @@ Record AsynchronousArena := {
     (polarity m = false -> finite_payoff_position nil = (1)%Z));
 
     polarity_second : forall m, second_move (P E) m -> 
-    ((polarity m = true -> finite_payoff_position nil = (-1)%Z)
+    ((polarity m = true -> finite_payoff_position nil = (1)%Z)
     /\
-    (polarity m = false -> finite_payoff_position nil = (1)%Z));
+    (polarity m = false -> finite_payoff_position nil = (-1)%Z));
 
     initial_null : forall (w : Walk E),
-    (valid_walk E w /\ snd (fst w) = nil /\ snd (snd w) = nil) -> 
+    (snd (fst w) = nil /\ snd (snd w) = nil) -> 
     finite_payoff_walk w = 0%Z;
 
     (*noninitial_payoff : forall (w : Walk E) (p : Position E),
-    (valid_walk E w /\
-    ((length (snd (fst w)) > 0) \/  (length (snd (fst w)) > 0)) /\ 
+    (((length (snd (fst w)) > 0) \/  (length (snd (fst w)) > 0)) /\ 
     (fst (fst w)) = nil) -> 
     finite_payoff_walk w = 
     finite_payoff_position ((fst (snd w)) ++ (snd (snd w)));*)
@@ -141,3 +142,111 @@ Record AsynchronousGame  :=
     leq (P (E A)) m n -> n = action (id X) n h)) -> 
     m = action (id X) m h
 }.
+
+Fact inverse_is_unique (G: Group) : forall x y z,
+mult G x y = id G /\ mult G x z = id G -> y = z.
+Proof. intros. destruct H. rewrite <- H in H0.
+assert (mult G (inverse G x) (mult G x z) = 
+mult G (inverse G x) (mult G x y) ).
+{  rewrite H0. reflexivity. }
+rewrite associative in H1. rewrite associative in H1.
+assert (mult G (inverse G x) x = id G).
+{ apply inverses_exist. }
+rewrite H2 in H1. 
+assert (mult G (id G) z = z /\ mult G (id G) y = y).
+{ split. 
++ apply id_exists.
++ apply id_exists. }
+destruct H3. rewrite H3 in H1. rewrite H4 in H1. auto.
+Qed.
+
+Fact mult_inverse (G: Group) : forall g g',
+mult G (inverse G g') (inverse G g) = inverse G (mult G g g').
+Proof. intros. 
+assert (mult G (mult G g g') (mult G (inverse G g') (inverse G g)) = id G /\
+mult G (mult G g g') (inverse G (mult G g g')) = id G).
+{ assert (mult G (mult G g g') (inverse G (mult G g g')) = id G).
+{ apply inverses_exist. }
+assert (mult G (mult G g g') (mult G (inverse G g') (inverse G g)) = id G).
+{ rewrite associative. 
+assert (mult G (mult G g g') (inverse G g') = g).
+{ rewrite <- associative.
+assert (mult G g' (inverse G g') = id G).
+{ apply inverses_exist. }
+rewrite H0. apply id_exists.
+  }
+rewrite H0. apply inverses_exist.
+ }
+rewrite H. rewrite H0. auto.
+} apply inverse_is_unique with (G0:=G) (x:=mult G g g')
+(y:=mult G (inverse G g') (inverse G g)) (z:=inverse G (mult G g g')).
+auto.
+Qed.
+
+Fact inverse_id_is_id (G: Group) : inverse G (id G) = id G.
+Proof. apply inverse_is_unique with (G0:=G) (x:=id G) 
+(y:= inverse G (id G)) (z:=id G). 
+split.
++ apply inverses_exist.
++ apply id_exists.
+Qed.
+
+Definition trivial_group : Group.
+refine({|
+          G := unit;
+          mult a b := tt;
+          id := tt
+      |}).
+Proof.
+- auto.
+- auto.
+- intros. destruct x. auto.
+- auto.
+Defined.
+
+Definition product_group (X Y : Group) : Group.
+refine ({|
+        G := (G X) * (G Y);
+        mult m n := (mult _ (fst m) (fst n), mult _ (snd m) (snd n));
+        id := (id _, id _);
+        inverse m := (inverse _ (fst m), inverse _ (snd m))
+       |}).
+Proof.
+- intros. destruct x. destruct y. destruct z. simpl.
+rewrite associative. rewrite associative. reflexivity.
+- intros. destruct x. simpl.
+assert (mult _ (id _) g = g /\ mult _ g (id _) = g).
+{ apply id_exists. }
+assert (mult _ (id _) g0 = g0 /\ mult _ g0 (id _) = g0).
+{ apply id_exists. }
+destruct H0. destruct H. rewrite H. rewrite H1. rewrite H0. rewrite H2. auto.
+- intros. destruct x. simpl. 
+assert (mult _ g (inverse _ g) = id _ /\ mult _ (inverse _ g) g = id _).
+{ apply inverses_exist. }
+assert (mult _ g0 (inverse _ g0) = id _ /\ mult _ (inverse _ g0) g0 = id _).
+{ apply inverses_exist. }
+destruct H. destruct H0. rewrite H. rewrite H1. rewrite H0. rewrite H2. auto.
+Defined.
+
+Definition valid_position (E : EventStructure) (p : Position E) :=
+forall m n, (In n p -> leq (P E) m n -> In m p)
+/\
+(In m p /\ In n p ->  not (incompatible E m n)).
+
+Definition move_from (E : EventStructure) (m : (M (P E))) (p q: Position E) :=
+(In m q) /\ (~ In m p) /\ (forall n, In n p -> In n q).
+
+Definition valid_path (E: EventStructure) (p : Path E) :=
+forall n, 0 <= n <= length (snd p) ->
+(valid_position E ((fst p) ++ (firstn n (snd p))) /\
+(n > 0 -> (exists m, (nth_error (snd p) (n-1)) = Some m /\
+move_from E m ((fst p) ++ (firstn (n-1) (snd p)))
+((fst p) ++ (firstn n (snd p)))))).
+
+Definition valid_walk (E: EventStructure) (w : Walk E) := 
+valid_path E (fst w) /\ valid_path E (snd w) /\
+(forall x,  In x (fst (fst w)) <-> In x (fst (snd w))).
+
+
+
+
