Tensor Product.v
@@ -103,21 +103,17 @@ assert (leq Q
 (existT (fun i : I Q => (unit + N Q i)%type) j0 (inr m0))). auto. }
 apply leq_tensor_right with (i:=i0) (j:=j0) (m:=m) (m':=m'0). auto.
 auto. auto.
+- intros. destruct i. unfold iff. split.
++ intros. inversion H.
+++ auto.
+++ subst. inversion H1.
+++ subst. inversion H1.
++ intros. subst. apply leq_tensor_least with (m:=m).
+- intros. inversion H.
++ auto.
++ subst. inversion H1. inversion H2. subst. auto.
++ subst. inversion H1. inversion H2. subst. auto.
 Defined.
-
-Record EventStructure := 
-  {
-    P : PartialOrder;
-    incompatible : (M P) -> (M P) -> Prop;
-
-    ideal : (M P)  -> list (M P);
-
-    symmetric : forall x y, incompatible x y -> incompatible y x;
-    irreflexive : forall x, not (incompatible x x);
-    ideal_finite : forall x y, leq P y x <-> In y (ideal x);
-    incompatible_closed : forall x y z,
-        (incompatible x y) /\ (leq P y z) -> incompatible x z
-  }.
 
 Inductive incompatible_tensor (E F : EventStructure) :
 (M (partial_order_tensor (P E) (P F))) ->
@@ -141,21 +137,21 @@ incompatible_tensor E F a b.
 
 Definition event_structure_tensor (E F : EventStructure) : EventStructure.
   refine({| 
-P := partial_order_tensor (P E) (P F);
-incompatible := incompatible_tensor E F;
-ideal m := match m with
-| existT _ (i, j) (inl tt) => (existT _ (i, j) (inl tt)) :: nil
-| existT _ (i, j) (inr (inl m)) =>
-map (fun x => match x with
-| existT _ i (inl tt) => existT _ (i, j) (inl tt)
-| existT _ i (inr m) => existT _ (i, j) (inr (inl m))
-end) (ideal E (existT _ i (inr m)))
-| existT _ (i, j) (inr (inr m)) =>
-map (fun x => match x with
-| existT _ j (inl tt) => existT _ (i, j) (inl tt)
-| existT _ j (inr m) => existT _ (i, j) (inr (inr m))
-end) (ideal F (existT _ j (inr m)))
-end;
+            P := partial_order_tensor (P E) (P F);
+            incompatible := incompatible_tensor E F;
+            ideal m := match m with
+                      | existT _ (i, j) (inl tt) => (existT _ (i, j) (inl tt)) :: nil
+                      | existT _ (i, j) (inr (inl m)) =>
+                      map (fun x => match x with
+                                    | existT _ i (inl tt) => existT _ (i, j) (inl tt)
+                                    | existT _ i (inr m) => existT _ (i, j) (inr (inl m))
+                      end) (ideal E (existT _ i (inr m)))
+                      | existT _ (i, j) (inr (inr m)) =>
+                      map (fun x => match x with
+                                    | existT _ j (inl tt) => existT _ (i, j) (inl tt)
+                                    | existT _ j (inr m) => existT _ (i, j) (inr (inr m))
+                                    end) (ideal F (existT _ j (inr m)))
+                      end;
          |}).
 Proof.
 - intros. inversion H.
@@ -193,4 +189,493 @@ assert (~ incompatible F
 + destruct x. destruct y.
 ++ destruct x. destruct s.
 +++ simpl. destruct u.
-++++
+++++ unfold iff. split.
++++++ intros. simpl. left. inversion H.
+++++++ subst. apply inj_pairT2 in H6. subst.
+apply inj_pairT2 in H3. subst. auto.
+++++++ subst. inversion H2.
+++++++ subst. inversion H2.
++++++ intros. destruct H.
+++++++ inversion H. subst. apply inj_pairT2 in H. subst.
+apply leq_tensor_least.
+++++++ contradiction H.
++++ destruct n.
+++++ simpl. unfold iff. split.
++++++ intros. apply in_map_iff. inversion H.
+++++++ subst. inversion H6. subst. 
+apply inj_pairT2 in H3. subst.
+refine (ex_intro _ (existT _ i (inl tt)) _). split.
++++++++ auto.
++++++++ apply ideal_finite. apply unit_is_least. auto.
+++++++ subst. inversion H2. subst. apply inj_pairT2 in H2.
+inversion H2. subst. inversion H1. subst. apply inj_pairT2 in H1.
+subst. refine (ex_intro _ (existT _ i3 (inr m)) _). split.
++++++++ auto.
++++++++ apply ideal_finite. auto.
+++++++ subst. inversion H2.
++++++ intros. apply in_map_iff in H. destruct H. destruct x. destruct s.
+++++++ destruct u. inversion H. subst. inversion H0. subst.
+apply inj_pairT2 in H0. subst. apply ideal_finite in H1. 
+apply unit_is_least in H1. subst. apply leq_tensor_least.
+++++++ destruct H. inversion H. subst. apply inj_pairT2 in H. subst.
+apply ideal_finite in H0. assert (H1 := H0).
+apply leq_same_component in H0. subst.
+apply leq_tensor_left with (i:=i) (j:=i2) (m:=n0) (m':=n). auto. auto.
+auto.
+++++ unfold iff. split.
++++++ intros. apply in_map_iff. inversion H.
+++++++ subst. apply inj_pairT2 in H3. subst.
+refine (ex_intro _ (existT _ i0 (inl tt)) _). split.
++++++++ auto.
++++++++ apply ideal_finite. apply unit_is_least. auto.
+++++++ subst. inversion H1. subst. apply inj_pairT2 in H1. subst.
+inversion H2.
+++++++ subst. inversion H2. subst. apply inj_pairT2 in H2. inversion H2.
+subst. inversion H1. subst. apply inj_pairT2 in H7. subst.
+refine (ex_intro _ (existT _ j (inr m)) _). split.
++++++++ auto.
++++++++ apply ideal_finite. auto.
++++++ intros.
+++++++ apply in_map_iff in H. destruct H. destruct x. destruct H. 
+apply ideal_finite in H0. assert (H1 := H0). apply leq_same_component in H0. subst.
+destruct s. 
++++++++ destruct u. inversion H. subst. apply inj_pairT2 in H. subst.
+apply leq_tensor_least.
++++++++ inversion H. subst. apply inj_pairT2 in H. subst.
+apply leq_tensor_right with (i:=i1) (j:=i2) (m:=n0) (m':=n). auto. auto. auto.
+- intros. destruct H. inversion H.
++ subst. inversion H0.
+++ apply incomp_tensor_least. auto.
+++ subst. inversion H3. subst. apply incomp_tensor_least. auto.
+++ subst. inversion H3. subst. apply incomp_tensor_least. auto.
++ subst. inversion H0.
+++ subst. inversion H3. subst. apply inj_pairT2 in H3. inversion H3.
+subst. apply incomp_tensor_left with (m:=m) (m':=m'0). apply incompatible_closed
+with (y:=(existT (fun i0 : I (P E) => (unit + N (P E) i0)%type)
+     (fst (i, j)) (inr m0))). auto. auto. auto.
+++ subst. inversion H3.
++ subst. inversion H0.
+++ subst. inversion H3.
+++ subst. inversion H3. subst. apply inj_pairT2 in H3. inversion H3.
+subst. apply incomp_tensor_right with (m:=m) (m':=m'0). apply incompatible_closed
+with (y:=(existT (fun i0 : I (P F) => (unit + N (P F) i0)%type)
+     (snd (i, j)) (inr m0))). auto. auto. auto.
+Defined.
+
+Fixpoint cast_tensor_to_left E F (l : Position (event_structure_tensor E F))
+: Position E :=
+match l with
+| nil => nil
+| (existT _ (i,j) (inl tt)) :: xs
+=> (existT _ i (inl tt)) :: (cast_tensor_to_left E F xs)
+| (existT _ (i,j) (inr (inl m))) :: xs
+=> (existT _ i (inr m)) :: (cast_tensor_to_left E F xs)
+| (existT _ i (inr (inr _))) :: xs
+=> cast_tensor_to_left E F xs
+end.
+
+Fixpoint cast_tensor_to_right E F (l : Position (event_structure_tensor E F))
+: Position F :=
+match l with
+| nil => nil
+| (existT _ (i,j) (inl tt)) :: xs
+=> (existT _ j (inl tt)) :: (cast_tensor_to_right E F xs)
+| (existT _ (i,j) (inr (inr m))) :: xs
+=> (existT _ j (inr m)) :: (cast_tensor_to_right E F xs)
+| (existT _ i (inr (inl _))) :: xs
+=> cast_tensor_to_right E F xs
+end.
+
+Fixpoint cast_tensor_inf_to_left E F (l : InfinitePosition (event_structure_tensor E F))
+: InfinitePosition E :=
+match l with
+| stream _ (existT _ (i, j) (inl tt)) f =>
+stream _ (existT _ i (inl tt)) (fun _ => cast_tensor_inf_to_left E F (f tt))
+| stream _ (existT _ (i, j) (inr (inl m))) f =>
+stream _ (existT _ i (inr m)) (fun _ => cast_tensor_inf_to_left E F (f tt))
+| stream _ (existT _ (i, j) (inr (inr _))) f =>
+cast_tensor_inf_to_left E F (f tt)
+end.
+
+Fixpoint cast_tensor_inf_to_right E F (l : InfinitePosition (event_structure_tensor E F))
+: InfinitePosition F :=
+match l with
+| stream _ (existT _ (i, j) (inl tt)) f =>
+stream _ (existT _ j (inl tt)) (fun _ => cast_tensor_inf_to_right E F (f tt))
+| stream _ (existT _ (i, j) (inr (inr m))) f =>
+stream _ (existT _ j (inr m)) (fun _ => cast_tensor_inf_to_right E F (f tt))
+| stream _ (existT _ (i, j) (inr (inl _))) f =>
+cast_tensor_inf_to_right E F (f tt)
+end.
+
+Definition tensor (p q : Z) :=
+if Z.ltb p 0 then 
+(if Z.ltb q 0 then Z.add p q else p)
+else
+(if Z.ltb q 0 then q else Z.add p q).
+
+Definition tensor_infinity (p q : Infinity) :=
+match p, q with
+| plus_infinity, plus_infinity => plus_infinity
+| _, _ => minus_infinity
+end.
+
+Fact initial_is_unit :
+forall E m, initial_move E m <->
+(exists i, m = existT _ i (inl tt)).
+Proof. unfold iff. split.
++ intros. unfold initial_move in H. destruct m. 
+refine (ex_intro _ x _). symmetry. apply H.
+apply unit_is_least. auto.
++ intros. unfold initial_move. intros. destruct H. subst.
+apply anti_symmetric. split.
+++ auto.
+++ destruct n. apply leq_same_component in H0. subst. 
+apply unit_is_least. auto.
+Qed.
+
+Fact second_in_tensor_is_second :
+forall E F m, second_move (P (event_structure_tensor E F)) m <->
+((exists i j k, m = existT _ (i,j) (inr (inl k)) /\ 
+second_move (P E) (existT _ i (inr k)))
+\/
+(exists i j k, m = existT _ (i,j) (inr (inr k)) /\ 
+second_move (P F) (existT _ j (inr k)))).
+Proof. unfold iff. split.
++ intros. unfold second_move in H. destruct H.
+rewrite initial_is_unit in H. destruct m. destruct s.
+++ contradiction H. refine (ex_intro _ x _). destruct u. auto.
+++ destruct x. destruct n.
++++ left. refine (ex_intro _ i _). refine (ex_intro _ i0 _).
+refine (ex_intro _ n _). split.
+++++ auto.
+++++ unfold second_move. unfold not. intros. split.
++++++ intros. rewrite initial_is_unit in H1. destruct H1.
+inversion H1.
++++++ intros. destruct n0.
+++++++ destruct s.
++++++++ destruct u. apply initial_is_unit.
+refine (ex_intro _ x _). auto.
++++++++ destruct H1. assert (H3 := H1).
+apply leq_same_component in H3. subst.
+assert (initial_move (P (event_structure_tensor E F))
+(existT
+          (fun i : I (P (event_structure_tensor E F)) =>
+           (unit + N (P (event_structure_tensor E F)) i)%type)
+          (i, i0) (inr (inl n0)))).
+{apply H0. split.
++ apply leq_tensor_left with (i:=i) (j:=i0) (m:=n0) (m':=n).
+++ auto.
+++ auto.
+++ auto.
++ unfold not. intros. apply inj_pairT2 in H3. inversion H3. subst.
+contradiction H2. auto. }
+apply initial_is_unit in H3. destruct H3. inversion H3.
++++ simpl. right. refine (ex_intro _ i _). refine (ex_intro _ i0 _).
+refine (ex_intro _ n _). split.
+++++ auto.
+++++ unfold second_move. split.
++++++ unfold not. intros. apply initial_is_unit in H1. destruct H1.
+inversion H1.
++++++ intros. destruct H1. assert (H3 := H1). destruct n0.
+++++++ apply leq_same_component in H3. subst. destruct s.
++++++++ apply initial_is_unit. destruct u. refine (ex_intro _ i0 _).
+auto.
++++++++
+assert (initial_move (P (event_structure_tensor E F))
+(existT
+          (fun i : I (P (event_structure_tensor E F)) =>
+           (unit + N (P (event_structure_tensor E F)) i)%type)
+          (i, i0) (inr (inr n0)))).
+{apply H0. split.
++ apply leq_tensor_right with (i:=i) (j:=i0) (m:=n0) (m':=n).
+++ auto.
+++ auto.
+++ auto.
++ unfold not. intros. apply inj_pairT2 in H3. inversion H3. subst.
+contradiction H2. auto.
+ } apply initial_is_unit in H3. destruct H3. inversion H3.
++ intros. destruct H. 
+++ destruct H. destruct H. destruct H. destruct H. subst. unfold second_move.
+split.
++++ unfold not. intros. apply initial_is_unit in H. destruct H. inversion H.
++++ intros. destruct H. unfold second_move in H0. destruct H0. destruct n.
+++++ destruct s.
++++++ apply initial_is_unit. destruct u. refine (ex_intro _ x2 _). auto.
++++++ inversion H.
+++++++ subst. inversion H5. subst. apply inj_pairT2 in H5. inversion H5.
+subst. inversion H4. subst. apply inj_pairT2 in H4. inversion H4. subst.
+assert (initial_move (P E) (existT (fun i : I (P E) => (unit + N (P E) i)%type) i
+          (inr m))).
+{apply H2. split.
++ auto.
++ unfold not. intros. apply inj_pairT2 in H6. inversion H6. subst. contradiction H1. auto.
+} apply initial_is_unit in H6. destruct H6. inversion H6.
+++++++ subst. inversion H5.
+++ destruct H. destruct H. destruct H. destruct H. subst. unfold second_move. split.
++++ unfold not. intros. apply initial_is_unit in H. destruct H. inversion H.
++++ intros. destruct H. unfold second_move in H0. destruct H0. destruct n.
+++++ destruct s.
++++++ apply initial_is_unit. destruct u. refine (ex_intro _ x2 _). auto.
++++++ inversion H.
+++++++ subst. inversion H5.
+++++++ subst. inversion H5. subst. apply inj_pairT2 in H5. inversion H5.
+subst. inversion H4. subst. apply inj_pairT2 in H4. inversion H4. subst.
+assert (initial_move (P F) (existT (fun i : I (P F) => (unit + N (P F) i)%type) j
+          (inr m))).
+{apply H2. split.
++ auto.
++ unfold not. intros. apply inj_pairT2 in H6. inversion H6. subst. contradiction H1. auto.
+} apply initial_is_unit in H6. destruct H6. inversion H6.
+Qed. 
+
+Definition asynchronous_arena_tensor (A B : AsynchronousArena) 
+(positive1 : (finite_payoff_position A) nil = (-1)%Z)
+(positive2 : (finite_payoff_position B) nil = (-1)%Z)
+: AsynchronousArena.
+  refine({| 
+            E := event_structure_tensor (E A) (E B);
+            polarity m := match m with
+                          | existT _ (i,j) (inl ll) => true
+                          | existT _ (i,j) (inr (inl m)) => (polarity A) (existT _ i (inr m))
+                          | existT _ (i,j) (inr (inr m)) => (polarity B) (existT _ j (inr m))
+                          end;
+            finite_payoff_position l :=
+              (match l with
+                | nil => (-1)%Z
+                | _ => let left := finite_payoff_position A (cast_tensor_to_left _ _ l) in
+                       let right := finite_payoff_position B (cast_tensor_to_right _ _ l) in
+                       tensor left right
+              end);
+            finite_payoff_walk w :=
+              let fp := cast_tensor_to_left _ _ (fst (fst w)) in
+              let fm := cast_tensor_to_left _ _ (snd (fst w)) in
+              let sp := cast_tensor_to_left _ _ (fst (snd w)) in
+              let sm := cast_tensor_to_left _ _ (snd (snd w)) in
+              let left := finite_payoff_walk A ((fp, fm), (sp, sm)) in
+              let fp := cast_tensor_to_right _ _ (fst (fst w)) in
+              let fm := cast_tensor_to_right _ _ (snd (fst w)) in
+              let sp := cast_tensor_to_right _ _ (fst (snd w)) in
+              let sm := cast_tensor_to_right _ _ (snd (snd w)) in
+              let right := finite_payoff_walk B ((fp, fm), (sp, sm)) in
+              tensor left right;
+            infinite_payoff l :=
+              let left := infinite_payoff A (cast_tensor_inf_to_left _ _ l) in
+              let right := infinite_payoff B (cast_tensor_inf_to_right _ _ l) in
+              tensor_infinity left right;
+         |}).
+Proof.
+- left. auto.
+- intros. apply initial_is_unit in H. destruct H. subst.
+destruct x. easy.
+- intros. apply second_in_tensor_is_second in H. destruct H.
++ destruct H. destruct H. destruct H. destruct H. subst. apply polarity_second in H0.
+rewrite positive1 in H0. auto.
++ destruct H. destruct H. destruct H. destruct H. subst. apply polarity_second in H0.
+rewrite positive2 in H0. auto.
+- intros. destruct H. destruct w. destruct p. destruct p0. simpl in *. subst. simpl.
+assert ((finite_payoff_walk A
+     (cast_tensor_to_left (E A) (E B) p, nil,
+     (cast_tensor_to_left (E A) (E B) p0, nil))) = 0%Z).
+{apply initial_null. auto. }
+assert ((finite_payoff_walk B
+     (cast_tensor_to_right (E A) (E B) p, nil,
+     (cast_tensor_to_right (E A) (E B) p0, nil))) = 0%Z).
+{apply initial_null. auto. }
+assert (forall a b f, a = 0%Z /\ b = 0%Z /\ f 0%Z 0%Z  = 0%Z
+-> f a b = 0%Z).
+{intros. destruct H1. destruct H2. subst. auto. }
+apply H1. auto.
+Defined.
+
+Definition asynchronous_game_tensor (G H: AsynchronousGame) 
+(pos1 : (finite_payoff_position (A G)) nil = (-1)%Z)
+(pos2 : (finite_payoff_position (A H)) nil = (-1)%Z)
+: AsynchronousGame.
+  refine({| 
+             A := asynchronous_arena_tensor (A G) (A H) pos1 pos2;
+             X := product_group (X G) (X H);
+             Y := product_group (Y G) (Y H);
+             action g m h := match m with
+                                | existT _ _ (inl tt) => m
+                                | existT _ (i,j) (inr (inl m)) => 
+                                  (match action G (fst g) (existT _ i (inr m)) (fst h) with
+                                    | existT _ i (inl tt) => existT _ (i,j) (inl tt)
+                                    | existT _ i (inr m) => existT _ (i,j) (inr (inl m))
+                                  end)
+                                | existT _ (i,j) (inr (inr m)) => 
+                                  (match action H (snd g) (existT _ j (inr m)) (snd h) with
+                                    | existT _ j (inl tt) => existT _ (i,j) (inl tt)
+                                    | existT _ j (inr m) => existT _ (i,j) (inr (inr m))
+                                  end)
+                             end;
+        |}).
+Proof.
+- intros. destruct m. destruct x. destruct s.
++ destruct u. auto.
++ destruct n.
+++ simpl in *. simpl. 
+remember ((let (i1, s) :=
+   action G (id (X G))
+     (existT (fun i1 : I (P (E (A G))) => (unit + N (P (E (A G))) i1)%type) i
+        (inr n)) (id (Y G)) in
+ match s with
+ | inl tt =>
+     existT
+       (fun i2 : I (P (E (A G))) * I (P (E (A H))) =>
+        (unit + (N (P (E (A G))) (fst i2) + N (P (E (A H))) (snd i2)))%type)
+       (i1, i0) (inl tt)
+ | inr m =>
+     existT
+       (fun i2 : I (P (E (A G))) * I (P (E (A H))) =>
+        (unit + (N (P (E (A G))) (fst i2) + N (P (E (A H))) (snd i2)))%type)
+       (i1, i0) (inr (inl m))
+ end)). 
+assert (forall A (a b c : A),
+a = b -> a = c -> b = c).
+{intros. subst. auto. }
+apply H0 with (a:=s).
++++ auto.
++++ destruct (action G (id (X G))
+            (existT (fun i1 : I (P (E (A G))) => (unit + N (P (E (A G))) i1)%type)
+               i (inr n)) (id (Y G))) eqn:eqn1. 
+++++ subst. rewrite action_id in eqn1. inversion eqn1. auto.
+++ simpl in *. simpl. remember ((let (j, s) :=
+   action H (snd (id (product_group (X G) (X H))))
+     (existT (fun i1 : I (P (E (A H))) => (unit + N (P (E (A H))) i1)%type) i0
+        (inr n)) (snd (id (product_group (Y G) (Y H)))) in
+ match s with
+ | inl tt =>
+     existT
+       (fun i1 : I (P (E (asynchronous_arena_tensor (A G) (A H) pos1 pos2))) =>
+        (unit + N (P (E (asynchronous_arena_tensor (A G) (A H) pos1 pos2))) i1)%type)
+       (i, j) (inl tt)
+ | inr m =>
+     existT
+       (fun i1 : I (P (E (asynchronous_arena_tensor (A G) (A H) pos1 pos2))) =>
+        (unit + N (P (E (asynchronous_arena_tensor (A G) (A H) pos1 pos2))) i1)%type)
+       (i, j) (inr (inr m))
+ end)).
+assert (forall A (a b c : A),
+a = b -> a = c -> b = c).
+{intros. subst. auto. }
+apply H0 with (a:=s).
++++ auto.
++++ destruct (action H (snd (id (product_group (X G) (X H))))
+            (existT (fun i1 : I (P (E (A H))) => (unit + N (P (E (A H))) i1)%type)
+               i0 (inr n)) (snd (id (product_group (Y G) (Y H))))) eqn:eqn1.
+++++ simpl in *. rewrite action_id in eqn1. inversion eqn1. subst. apply inj_pairT2 in H3.
+subst. auto.
+-  intros. destruct m. destruct g. destruct g'. destruct h. destruct h'. destruct x. simpl.
+destruct s.
++ destruct u. auto.
++ destruct n.
+++ remember ((let (i1, s) :=
+   action G (mult (X G) g g1)
+     (existT (fun i1 : I (P (E (A G))) => (unit + N (P (E (A G))) i1)%type) i
+        (inr n)) (mult (Y G) g3 g5) in
+ match s with
+ | inl tt =>
+     existT
+       (fun i2 : I (P (E (A G))) * I (P (E (A H))) =>
+        (unit + (N (P (E (A G))) (fst i2) + N (P (E (A H))) (snd i2)))%type)
+       (i1, i0) (inl tt)
+ | inr m =>
+     existT
+       (fun i2 : I (P (E (A G))) * I (P (E (A H))) =>
+        (unit + (N (P (E (A G))) (fst i2) + N (P (E (A H))) (snd i2)))%type)
+       (i1, i0) (inr (inl m))
+ end)).
+assert (forall A (a b c : A), a = b -> b = c -> a = c).
+{intros. subst. auto. }
+apply H0 with (b:=s). auto.
+remember ((let (x0, s0) :=
+   let (i1, s0) :=
+     action G g1
+       (existT (fun i1 : I (P (E (A G))) => (unit + N (P (E (A G))) i1)%type) i
+          (inr n)) g3 in
+   match s0 with
+   | inl tt =>
+       existT
+         (fun i2 : I (P (E (A G))) * I (P (E (A H))) =>
+          (unit + (N (P (E (A G))) (fst i2) + N (P (E (A H))) (snd i2)))%type)
+         (i1, i0) (inl tt)
+   | inr m =>
+       existT
+         (fun i2 : I (P (E (A G))) * I (P (E (A H))) =>
+          (unit + (N (P (E (A G))) (fst i2) + N (P (E (A H))) (snd i2)))%type)
+         (i1, i0) (inr (inl m))
+   end in
+ (let
+    (i1, j) as x1
+     return
+       (unit + (N (P (E (A G))) (fst x1) + N (P (E (A H))) (snd x1)) ->
+        M (partial_order_tensor (P (E (A G))) (P (E (A H))))) := x0 in
+  fun s1 : unit + (N (P (E (A G))) i1 + N (P (E (A H))) j) =>
+  match s1 with
+  | inl tt =>
+      let (i2, s2) :=
+        action G g1
+          (existT (fun i2 : I (P (E (A G))) => (unit + N (P (E (A G))) i2)%type)
+             i (inr n)) g3 in
+      match s2 with
+      | inl tt =>
+          existT
+            (fun i3 : I (P (E (A G))) * I (P (E (A H))) =>
+             (unit + (N (P (E (A G))) (fst i3) + N (P (E (A H))) (snd i3)))%type)
+            (i2, i0) (inl tt)
+      | inr m =>
+          existT
+            (fun i3 : I (P (E (A G))) * I (P (E (A H))) =>
+             (unit + (N (P (E (A G))) (fst i3) + N (P (E (A H))) (snd i3)))%type)
+            (i2, i0) (inr (inl m))
+      end
+  | inr (inl m) =>
+      let (i2, s2) :=
+        action G g
+          (existT (fun i2 : I (P (E (A G))) => (unit + N (P (E (A G))) i2)%type)
+             i1 (inr m)) g5 in
+      match s2 with
+      | inl tt =>
+          existT
+            (fun i3 : I (P (E (A G))) * I (P (E (A H))) =>
+             (unit + (N (P (E (A G))) (fst i3) + N (P (E (A H))) (snd i3)))%type)
+            (i2, j) (inl tt)
+      | inr m0 =>
+          existT
+            (fun i3 : I (P (E (A G))) * I (P (E (A H))) =>
+             (unit + (N (P (E (A G))) (fst i3) + N (P (E (A H))) (snd i3)))%type)
+            (i2, j) (inr (inl m0))
+      end
+  | inr (inr m) =>
+      let (j0, s2) :=
+        action H g0
+          (existT (fun i2 : I (P (E (A H))) => (unit + N (P (E (A H))) i2)%type)
+             j (inr m)) g6 in
+      match s2 with
+      | inl tt =>
+          existT
+            (fun i2 : I (P (E (A G))) * I (P (E (A H))) =>
+             (unit + (N (P (E (A G))) (fst i2) + N (P (E (A H))) (snd i2)))%type)
+            (i1, j0) (inl tt)
+      | inr m0 =>
+          existT
+            (fun i2 : I (P (E (A G))) * I (P (E (A H))) =>
+             (unit + (N (P (E (A G))) (fst i2) + N (P (E (A H))) (snd i2)))%type)
+            (i1, j0) (inr (inr m0))
+      end
+  end) s0)). symmetry.
+apply H0 with (b:=m). auto.
++++ destruct (action G (mult (X G) g g1)
+            (existT
+               (fun i1 : I (P (E (A G))) => (unit + N (P (E (A G))) i1)%type) i
+               (inr n)) (mult (Y G) g3 g5)) eqn:eqn1.
+++++ destruct s0.
++++++ destruct u. 
+destruct ( action G g1
+              (existT (fun i1 : I (P (E (A G))) => (unit + N (P (E (A G))) i1)%type) i
+                 (inr n)) g3) eqn:eqn2.
+++++++ destruct s0.
++++++++ destruct u. simpl in *. subst. rewrite action_compatible in eqn1.
+
+
